work around lack of fixpoint matching in coq<8.9

bedrock2/src/WeakestPrecondition.v
@@ -17,40 +17,42 @@ Section WeakestPrecondition.
 
   Section WithMemAndLocals.
     Context (m : mem) (l : locals).
-    Fixpoint expr (e : Syntax.expr) (post : word -> Prop) : Prop :=
+    Definition expr_body rec (e : Syntax.expr) (post : word -> Prop) : Prop :=
       match e with
       | expr.literal v =>
         literal v post
       | expr.var x =>
         get l x post
       | expr.op op e1 e2 =>
-        expr e1 (fun v1 =>
-        expr e2 (fun v2 =>
+        rec e1 (fun v1 =>
+        rec e2 (fun v2 =>
         post (interp_binop op v1 v2)))
       | expr.load s e =>
-        expr e (fun a =>
+        rec e (fun a =>
         load s m a post)
     end.
+    Fixpoint expr e := expr_body expr e.
   End WithMemAndLocals.
 
   Section WithF.
     Context {A B} (f: A -> (B -> Prop) -> Prop).
-    Fixpoint list_map (xs : list A) (post : list B -> Prop) {struct xs} : Prop :=
+    Definition list_map_body rec (xs : list A) (post : list B -> Prop) : Prop :=
       match xs with
       | nil => post nil
       | cons x xs' =>
         f x (fun y =>
-        list_map xs' (fun ys' =>
+        rec xs' (fun ys' =>
         post (cons y ys')))
       end.
+    Fixpoint list_map xs := list_map_body list_map xs.
   End WithF.
 
   Section WithFunctions.
     Context (call : funname -> trace -> mem -> list word -> (trace -> mem -> list word -> Prop) -> Prop).
     Definition dexpr m l e v := expr m l e (eq v).
     Definition dexprs m l es vs := list_map (expr m l) es (eq vs).
-    Fixpoint cmd (c : cmd) (t : trace) (m : mem) (l : locals)
-             (post : trace -> mem -> locals -> Prop) {struct c} : Prop :=
+    Definition cmd_body (rec:_->_->_->_->_->Prop) (c : cmd) (t : trace) (m : mem) (l : locals)
+             (post : trace -> mem -> locals -> Prop) : Prop :=
       (* give value of each pure expression when stating its subproof *)
       match c with
       | cmd.skip => post t m l
@@ -65,17 +67,17 @@ Section WeakestPrecondition.
         post t m l)
       | cmd.cond br ct cf =>
         bind_ex v <- dexpr m l br;
-        (word_test v = true  -> cmd ct t m l post) /\
-        (word_test v = false -> cmd cf t m l post)
+        (word_test v = true  -> rec ct t m l post) /\
+        (word_test v = false -> rec cf t m l post)
       | cmd.seq c1 c2 =>
-        cmd c1 t m l (fun t m l => cmd c2 t m l post)
+        rec c1 t m l (fun t m l => rec c2 t m l post)
       | cmd.while e c =>
         exists measure (lt:measure->measure->Prop) (inv:measure->trace->mem->locals->Prop), 
         Coq.Init.Wf.well_founded lt /\
         (exists v, inv v t m l) /\
         (forall v t m l, inv v t m l ->
           bind_ex b <- dexpr m l e;
-          (word_test b = true -> cmd c t m l (fun t' m l =>
+          (word_test b = true -> rec c t m l (fun t' m l =>
             exists v', inv v' t' m l /\ (progress t' t \/ lt v' v))) /\
           (word_test b = false -> post t m l))
       | cmd.call binds fname arges =>
@@ -90,6 +92,7 @@ Section WeakestPrecondition.
           guarantee t /\
           (rely t -> (bind_ex_Some l <- map.putmany binds rets l; post t m l))
       end.
+    Fixpoint cmd c := cmd_body cmd c.
   End WithFunctions.
 
   Definition func call '(innames, outnames, c) (t : trace) (m : mem) (args : list word) (post : trace -> mem -> list word -> Prop) :=
@@ -98,16 +101,17 @@ Section WeakestPrecondition.
         list_map (get l) outnames (fun rets =>
         post t m rets)).
           
-  Fixpoint call (functions : list (funname * (list varname * list varname * cmd.cmd)))
+  Definition call_body rec (functions : list (funname * (list varname * list varname * cmd.cmd)))
                 (fname : funname) (t : trace) (m : mem) (args : list word)
-                (post : trace -> mem -> list word -> Prop) {struct functions} : Prop :=
+                (post : trace -> mem -> list word -> Prop) : Prop :=
     match functions with
     | nil => False
     | cons (f, decl) functions =>
       if funname_eqb f fname
-      then func (call functions) decl t m args post
-      else call functions fname t m args post
+      then func (rec functions) decl t m args post
+      else rec functions fname t m args post
     end.
+  Fixpoint call functions := call_body call functions.
 
   Definition program funcs main t m l post : Prop := cmd (call funcs) main t m l post.
 End WeakestPrecondition.
